lean/src/u_eval_theorem.lean
@@ -1,12 +1,102 @@
+import tactic
 import .defs
+import .lemmas
 
 variable [GuardModule]
 open GuardModule
 
+def as_no_match : Result → option Env
+| (Result.no_match env) := some env
+| (Result.diverged) := none
+| (Result.leaf _) := none
+
+
 -- Uncovered refinement types capture all values that are not covered.
 -- This theorem might be easier to show for 𝒰' rather than 𝒰.
 theorem 𝒰_eval :
-    ∀ env: Env, ∀ gdt: Gdt,
-        (gdt_eval gdt env ≠ Result.no_match) ↔ (Φ_eval (𝒰 gdt) env = none)
-    := sorry
+    ∀ gdt: Gdt, ∀ env: Env,
+        as_no_match (gdt_eval gdt env) = Φ_eval (𝒰 gdt) env := 
+begin
+    assume gdt: Gdt,
+    assume env: Env,
 
+    rw 𝒰_𝒰'_equiv,
+ 
+    induction gdt with leaf generalizing env,
+
+    case Gdt.leaf {
+        unfold gdt_eval,
+        unfold 𝒰',
+        unfold Φ_eval,
+        finish,
+    },
+  
+    case Gdt.branch {
+        unfold 𝒰',
+        unfold gdt_eval,
+        unfold Φ_eval,
+        simp,
+
+        cases c1: (Φ_eval (𝒰' gdt_tr1) env),
+
+        all_goals {
+            rw Φ_eval._match_3,
+            specialize gdt_ih_tr1 env,
+            rw c1 at gdt_ih_tr1,
+            cases gdt_eval gdt_tr1 env,
+        },
+
+        all_goals {
+            rw gdt_eval._match_1,
+        },
+        repeat {
+            finish,
+        },
+
+        rw as_no_match at gdt_ih_tr1,
+        simp at gdt_ih_tr1,
+        finish
+    },
+
+    case Gdt.grd {
+        cases gdt_grd,
+        all_goals {
+            unfold 𝒰',
+            unfold gdt_eval,
+            unfold Φ_eval,
+            simp
+        },
+
+        {
+            cases (xgrd_eval gdt_grd env),
+            all_goals {
+                rw gdt_eval._match_2,
+                rw Φ_eval._match_1,
+                rw Φ_eval._match_3,
+                rw Φ_eval._match_2,
+            },
+            {
+                rw as_no_match,
+            },
+            {
+                specialize gdt_ih val,
+                exact gdt_ih,
+            }
+        },
+
+        {
+            cases (is_bottom gdt_grd env),
+            all_goals {
+                simp,
+                unfold Φ_eval._match_3,
+            },
+            {
+                specialize gdt_ih env,
+                exact gdt_ih,
+            },
+            {
+                finish,
+            }
+        }
+    }
+end
